debundle Bedrock, feeble attempts at Fixpoint evaluation

Analysis.v
@@ -1,12 +1,14 @@
-Require Import List.
+Require Import String.
 Require Import Div2.
 Require Import Bool.
+Require Import List.
+Require Vector.
 
-Require Import Word.
+Import ListNotations.
+
+Require Word.
 Require Import Parser.
-Require Import Datatypes.
-Require IL.
-Require NatMap.
+
 
 (*
      "Each instruction performs some action on the pseudo-machine state, which
@@ -15,127 +17,247 @@ Require NatMap.
         -OpenBSD man page
 *)
 
-Record state : Type := make_state {
-    prev_instrs : list instr;
+
+Definition scratch_mem := Vector.t (option (Word.word 32)) 16.
+
+Definition empty_mem : scratch_mem :=
+    Vector.const (None : option (Word.word 32)) 16.
+
+Record vm_state : Type := make_state {
     curr_instr : instr;
-    next_instrs : list instr;
-    acc : imm;
-    x_reg : imm;
-    pkt : list imm;
-    smem : list imm
+    (* Future instructions kept separate for ease of Fixpoint defs *)
+    acc : option imm;
+    x_reg : option imm;
+    pkt : scratch_mem;
+    smem : scratch_mem
 }.
 
-Definition step (s : state) : option state :=
+Inductive end_state : Type :=
+    | Ret : Word.word 32 -> end_state
+    | Error : string -> end_state.
+
+Inductive state : Type :=
+    | ContState : vm_state -> state
+    | End : end_state -> state.
+
+Definition init_state (ins : list instr) : state :=
+    match hd_error ins with
+        | None =>
+            End (Error "empty instruction list")
+        | Some i =>
+            ContState (make_state i None None empty_mem empty_mem)
+    end.
+
+
+
+Definition step (s : vm_state) : state * nat :=
     match curr_instr s with
         | SoloInstr s_op =>
             match s_op with
                 | RetA =>
-                    None
+                    (End (Error "*** fill in ***"), 1)
                 | RetK =>
-                    None
+                    (End (Error "*** fill in ***"), 1)
                 | XStoreA =>
-                    None
+                    (End (Error "*** fill in ***"), 1)
                 | AStoreX =>
-                    None
+                    (End (Error "*** fill in ***"), 1)
                 | LdXHdrLen =>
-                    None
+                    (End (Error "*** fill in ***"), 1)
                 | LdLen =>
-                    None
+                    (End (Error "*** fill in ***"), 1)
                 | LdXLen =>
-                    None
+                    (End (Error "*** fill in ***"), 1)
             end
         | ImmInstr i_op i =>
             match i_op with
                 | LdImm =>
-                    None
+                    (End (Error "*** fill in ***"), 1)
                 | AddImm =>
-                    None
+                    (End (Error "*** fill in ***"), 1)
                 | SubImm =>
-                    None
+                    (End (Error "*** fill in ***"), 1)
                 | MulImm =>
-                    None
+                    (End (Error "*** fill in ***"), 1)
                 | DivImm =>
-                    None
+                    (End (Error "*** fill in ***"), 1)
                 | AndImm =>
-                    None
+                    (End (Error "*** fill in ***"), 1)
                 | OrImm =>
-                    None
+                    (End (Error "*** fill in ***"), 1)
                 | SLImm =>
-                    None
+                    (End (Error "*** fill in ***"), 1)
                 | SRImm =>
-                    None
+                    (End (Error "*** fill in ***"), 1)
                 | AddX =>
-                    None
+                    (End (Error "*** fill in ***"), 1)
                 | SubX =>
-                    None
+                    (End (Error "*** fill in ***"), 1)
                 | MulX =>
-                    None
+                    (End (Error "*** fill in ***"), 1)
                 | DivX =>
-                    None
+                    (End (Error "*** fill in ***"), 1)
                 | AndX =>
-                    None
+                    (End (Error "*** fill in ***"), 1)
                 | OrX =>
-                    None
+                    (End (Error "*** fill in ***"), 1)
                 | SLX =>
-                    None
+                    (End (Error "*** fill in ***"), 1)
                 | SRX =>
-                    None
+                    (End (Error "*** fill in ***"), 1)
                 | Neg =>
-                    None
+                    (End (Error "*** fill in ***"), 1)
                 | JmpImm =>
-                    None
+                    (End (Error "*** fill in ***"), 1)
                 | LdXImm =>
-                    None
+                    (End (Error "*** fill in ***"), 1)
             end
         | MemInstr m_op m_addr =>
             match m_op with
                 | LdMem =>
-                    None
+                    (End (Error "*** fill in ***"), 1)
                 | LdXMem =>
-                    None
+                    (End (Error "*** fill in ***"), 1)
                 | Store =>
-                    None
+                    (End (Error "*** fill in ***"), 1)
                 | StoreX =>
-                    None
+                    (End (Error "*** fill in ***"), 1)
             end
         | PktInstr p_op p_addr =>
             match p_op with
                 | LdWord =>
-                    None
+                    (End (Error "*** fill in ***"), 1)
                 | LdHalf =>
-                    None
+                    (End (Error "*** fill in ***"), 1)
                 | LdByte =>
-                    None
+                    (End (Error "*** fill in ***"), 1)
                 | LdOfstWord =>
-                    None
+                    (End (Error "*** fill in ***"), 1)
                 | LdOfstHalf =>
-                    None
+                    (End (Error "*** fill in ***"), 1)
                 | LdXByte =>
-                    None
+                    (End (Error "*** fill in ***"), 1)
             end
         | BrInstr b_op ofst1 ofst2 =>
             match b_op with
                 | JGTX =>
-                    None
+                    (End (Error "*** fill in ***"), 1)
                 | JGEX =>
-                    None
+                    (End (Error "*** fill in ***"), 1)
                 | JEqX =>
-                    None
+                    (End (Error "*** fill in ***"), 1)
                 | JAndX =>
-                    None
+                    (End (Error "*** fill in ***"), 1)
             end
         | ImmBrInstr i_b_op i ofst1 ofst2 =>
             match i_b_op with
                 | JGTImm =>
-                    None
+                    (End (Error "*** fill in ***"), 1)
                 | JGEImm =>
-                    None
+                    (End (Error "*** fill in ***"), 1)
                 | JEqImm =>
-                    None
+                    (End (Error "*** fill in ***"), 1)
                 | JAndImm =>
-                    None
+                    (End (Error "*** fill in ***"), 1)
             end
     end.
+
+(*
+Fixpoint beq_nat (n m : nat) : bool :=
+  match n with
+  | O => match m with
+         | O => true
+         | S m' => false
+         end
+  | S n' => match m with
+            | O => false
+            | S m' => beq_nat n' m'
+            end
+  end.
+
+Definition beq_nat 
+
+Variable A : Type.
+Require Import Bool.
+Theorem not_zero : forall (n:nat), beq_nat (S n) 0 = false.
+simpl. reflexivity. Qed.
+
+Theorem skipn_dec : forall (n:nat) (l:list A), gt (length l) 0 -> lt (length (skipn (S n) l)) (length l).
+Proof.
+rewrite -> not_zero.
+simpl.
+intuition.
+rewrite -> not_zero.
+Qed.
+
+Variable A : Type.
+
+Definition lte (a b : nat) := or (lt a b) (eq a b).
+
+Lemma ref : forall (n:nat), eq n n.
+reflexivity.
+Qed.
+
+Lemma refl : forall (n:nat), lte n n.
+destruct n as [| n']. rewrite -> ref. reflexivity.
+Qed.
+
+Theorem skipn_dec : forall (n:nat) (l:list A), lte (length (skipn n l)) (length l).
+
+destruct n as [| n']. simpl. rewrite -> lte. reflexivity.*)
+
+Lemma skipn_dec : forall A (n:nat) (l:list A), length l >= length (skipn n l).
+Proof.
+intros A n l.
+induction l as [| hd tl].
+intro Hn.
+
+
+simpl.
+destruct n as [| n'].
+simpl.
+intuition.
+intuition.
+rewrite hi.
+
+intuition.
+destruct n as [| n'].
+simpl.
+intuition.
+simpl.
+case [].
+induction l.
+reflexivity.
+induction l.
+simpl.
+reflexivity.
+Qed.
+
+
+Fixpoint prog_eval (ins : list instr) (s : state) : end_state :=
+    match ins with
+        | next_i :: rest =>
+            match s with
+            | ContState vms =>
+                match step vms with
+                    | (_, 0) => Error "step size of zero"
+                    | (vms', step_size) => prog_eval rest vms'
+                end
+            | End end_s => end_s
+            end
+        | [] =>
+            Error "empty instr list, never reached a return"
+    end.
+(*
+    match s with
+        | ContState vms =>
+            match step vms with
+                | (_, 0) => Error "step size of zero"
+                | (vms', step_size) => prog_eval (skipn step_size ins) vms'
+            end
+        | End end_s =>
+            end_s
+    end.*)
 
 (* Used to prove that offsets stay on word (and hence instruction)
    boundaries.
@@ -143,9 +265,3 @@ Definition step (s : state) : option state :=
 
 Definition word_aligned sz (w : word sz) : bool :=
     (negb (mod2 (wordToNat w))) && (negb (mod2 (div2 (wordToNat w)))).
-
-(*
-Parameter mike_m : mem.
-Parameter mike_a : addr.
-Eval compute in (mem_get mike_m) mike_a.
-*)
