Makefile
@@ -10,26 +10,34 @@ VAL_FILES=validator/Alphabet.v \
 	validator/Interpreter_safe.v \
 	validator/Main.v
 
-COQ_DIRS=-I . -I validator -I includes -I bedrock
+COQ_DIRS=-I . -I validator -I includes -I bedrock/src
 
 all:
-	# necessary Bedrock libraries
-	coqc bedrock/Labels.v
-	coqc bedrock/Nomega.v
-	coqc bedrock/Reflection.v
-	coqc bedrock/EqdepClass.v
-	coqc bedrock/PropX.v
-	coqc -I bedrock bedrock/NatMap.v
-	coqc -I bedrock bedrock/Word.v
-	coqc -I bedrock bedrock/Memory.v
-	coqc -I bedrock bedrock/Decidables.v
-	coqc -I bedrock bedrock/DepList.v
-	coqc -I bedrock bedrock/Heaps.v
-	coqc -I bedrock bedrock/PropXTac.v
-	coqc -I bedrock bedrock/IL.v
-	coqc -I bedrock bedrock/SepTheoryX.v
-	coqc -I bedrock bedrock/SepTheoryXIL.v
-	coqc -I bedrock bedrock/SepIL.v
+	# independent Bedrock libraries
+	#coqc bedrock/Labels.v
+	#coqc bedrock/Nomega.v
+	#coqc bedrock/Reflection.v
+	#coqc bedrock/EqdepClass.v
+	# this one takes longer than the rest combined
+	#coqc bedrock/PropX.v
+	${MAKE} dependent
+
+dependent:
+	#coqc -I bedrock bedrock/Folds.v
+	#coqc -I bedrock bedrock/NatMap.v
+	#coqc -I bedrock bedrock/Word.v
+	#coqc -I bedrock bedrock/Memory.v
+	#coqc -I bedrock bedrock/Decidables.v
+	#coqc -I bedrock bedrock/DepList.v
+	#coqc -I bedrock bedrock/Expr.v
+	#coqc -I bedrock bedrock/Heaps.v
+	#coqc -I bedrock bedrock/PropXTac.v
+	#coqc -I bedrock bedrock/PropXRel.v
+	#coqc -I bedrock bedrock/IL.v
+	#coqc -I bedrock bedrock/SepTheoryX.v
+	#coqc -I bedrock bedrock/SepTheoryXIL.v
+	#coqc -I bedrock bedrock/SepExpr.v
+	#coqc -I bedrock bedrock/SepIL.v
 	# the CompCert parser validator
 	coqc -I validator ${VAL_FILES}
 	# includes from other parts of CompCert
@@ -42,10 +50,10 @@ all:
 incr:
 	ocamllex Lexer.mll
 	menhir --coq Parser.vy
-	coqc ${COQ_DIRS} Parser.v
-	coqc ${COQ_DIRS} Datatypes.v
-	coqc ${COQ_DIRS} Analysis.v
-	coqc ${COQ_DIRS} Extract.v
+	coqc ${COQ_DIRS} -R bedrock/src/ Bedrock Parser.v
+	coqc ${COQ_DIRS} -R bedrock/src/ Bedrock Datatypes.v
+	coqc ${COQ_DIRS} -R bedrock/src/ Bedrock Analysis.v
+	coqc ${COQ_DIRS} -R bedrock/src/ Bedrock Extract.v
 	#ocamlc -c Word.mli
 	#ocamlc -c Word.ml
 	ocamlc -c Parser.mli
@@ -60,5 +68,5 @@ clean:
 	rm -f *.glob *.cmi *.cmo a.out *.vo Parser.ml Lexer.ml \
 		Parser.v validator/*.{glob,vo} Main.ml \
 		Main.mli Parser.mli Lexer.mli Word.ml \
-		includes/*.cm{o,i} bedrock/*.{glob,vo} \
+		includes/*.cm{o,i} \
 		Analysis.ml{,i}
